EffectSSA/Semantics/Equiv/ProgramContext.lean
@@ -1,7 +1,9 @@
 import EffectSSA.Semantics.Environment
 import EffectSSA.Semantics.Program
 import EffectSSA.Semantics.Lemmas
+import EffectSSA.Semantics.TProgram
 import EffectSSA.Types
+import EffectSSA.Syntax.Typed
 
 import EffectSSA.Tactic.Typecheck
 
@@ -29,27 +31,90 @@ is implicitly between the two programs, where:
 - `pre` should be welltyped under the empty context
 - The return types of `pre` indicate the free variables available to the "hole"
 - The free variables of `post` indicate the expected return types of the "hole"
+
+Note: although this is not enforced in `ProgramContext`, the `post` program is
+expected to have exactly one return variable. Since we universally quantiy
+over context when defining contextual equivalence, we don't lose any expressive
+power by disallowing multiple return variables, but it does make things easier.
 -/
 structure ProgramContext τ : Type where
   pre  : Program τ
   post : Program τ
 
+/--
+A typed program context `TProgramContext Γ ts` bundles proofs that the "hole"
+of the context is shapped exactly like a `TProgram Γ ts`.
+-/
+structure TProgramContext (Γ : Context τ) (ts : List τ.Typ) where
+  ctx : ProgramContext τ
+  /--
+  The return type of the context (when filled).
+
+  Recall that we expect a program context to return only a single variable at the
+  end. Furthermore, an explicit goal of using contextual equivalence is to be able
+  to equate traces where events have been moved around in irrelvevant ways,
+  without having to explicitly define when that is the case. That is why we don't
+  want the precise structure of the trace to leak out of the context and thus we
+  mandate that the return type *must* be a plain data type.
+  -/
+  finalType : τ.DType
+  wt_pre : ctx.pre.WellTyped ∅ Γ.toList
+  wt_post : ctx.post.WellTyped ⟨ts⟩ [finalType]
+
+
+/-! ### Grind Attributes -/
+grind_pattern TProgramContext.wt_pre => (TProgramContext.ctx self).pre
+grind_pattern TProgramContext.wt_post => (TProgramContext.ctx self).post
+
 /-!
 ## API
 --------------------------------------------------------------------------------
 -/
-namespace ProgramContext
-variable {τ} [MemoryModel τ] {Δ : Context τ}
+variable {τ} {Γ Δ : Context τ}
+
+def TProgramContext.pre (C : TProgramContext Γ ts) : TProgram ∅ Γ.toList where
+  program := C.ctx.pre
+def TProgramContext.post (C : TProgramContext Γ ts) : TProgram ⟨ts⟩ [C.finalType] where
+  program := C.ctx.post
 
 /--
 Execute a program under the given context.
+That is, plug program `p` into the hole of context `C`, and evaluate the
+resulting program, returning `none` when the program is malformed, or has more
+than a single return variable.
+-/
+def ProgramContext.execProgram [MemoryModel τ] (C : ProgramContext τ) (p : Program τ) :
+    Option τ.Val := do
+  let (env, es) ← C.pre.execClosed
+  let (env, es) ← p.exec env es
+  let (env, _) ← C.post.exec env es
+  if env.size = 1 then
+    env.get? ⟨0⟩
+  else
+    none
+
+/--
+Execute a (typed) program under the given (typed) context.
 
 That is, plug program `p` into the hole of context `C`, and evaluate the
 resulting program.
 -/
-def execProgram (C : ProgramContext τ) (p : Program τ) :
-    Option (Environment τ) := do
-  let (env, es) ← C.pre.execClosed
-  let (env, es) ← p.exec env es
-  let (env, _) ← C.post.exec env es
-  return env
+def TProgramContext.execProgram [MemoryModel τ] (C : TProgramContext Γ ts) (p : TProgram Γ ts) :
+    τ.TVal C.finalType :=
+  let (env, es) := C.pre.execClosed
+  let (env, es) := p.exec env es
+  let (env, _) := C.post.exec env es
+  env.get ⟨⟨0⟩, rfl⟩
+
+/-!
+## Lemmas
+--------------------------------------------------------------------------------
+-/
+variable {ts} (C : TProgramContext Γ ts)
+
+@[simp, grind =] theorem TProgramContext.ctx_pre : C.ctx.pre = C.pre.program := by rfl
+@[simp, grind =] theorem TProgramContext.ctx_post : C.ctx.post = C.post.program := by rfl
+
+@[simp, grind =] theorem TProgramContext.ctx_exec_eq [MemoryModel τ] (p : TProgram Γ ts) :
+    C.ctx.execProgram p.program = some (C.execProgram p).toVal := by
+  simp [execProgram, ProgramContext.execProgram]
